WIP serialize dsum

src/lowparse/LowParse.SLow.Sum.fst
@@ -879,6 +879,95 @@ let parse32_dsum
 = fun input ->
   (parse32_dsum' t p32 f f32 g32 destr input <: (res: option (dsum_type t * U32.t) { parser32_correct (parse_dsum t p f g) input res } ))
 
+#set-options "--z3rlimit 32"
+
+let serialize32_dsum_aux
+  (#kt: parser_kind)
+  (t: dsum)
+  (#p: parser kt (dsum_repr_type t))
+  (s: serializer p)
+  (s32: serializer32 (serialize_maybe_enum_key _ s (dsum_enum t)))
+  (f: (x: dsum_known_key t) -> Tot (k: parser_kind & parser k (dsum_type_of_known_tag t x)))
+  (sf: (x: dsum_known_key t) -> Tot (serializer (dsnd (f x))))
+  (sf32: (x: dsum_known_key t) -> Tot (serializer32 (sf x)))
+  (#k': parser_kind)
+  (#g: parser k' (dsum_type_of_unknown_tag t))
+  (#sg: serializer g)
+  (sg32: serializer32 sg)
+  (u: squash (serializer32_sum_gen_precond kt (weaken_parse_dsum_cases_kind t f k')))
+: GTot (serializer32 (serialize_dsum t s f sf g sg))
+= fun x ->
+  serialize_dsum_eq t s f sf g sg x;
+  let tg = dsum_tag_of_data t x in
+  let s1 = s32 tg in
+  let s2 =
+    match tg with
+    | Known tg' -> sf32 tg' (synth_dsum_case_recip t tg x)
+    | Unknown _ -> sg32 (synth_dsum_case_recip t tg x)
+  in
+  assert (B32.length s1 + B32.length s2 < 4294967296);
+  let res = s1 `B32.b32append` s2 in
+  assert (serializer32_correct (serialize_dsum t s f sf g sg) x res);
+  (res <: (res: B32.bytes { serializer32_correct (serialize_dsum t s f sf g sg) x res } ))
+
+
+inline_for_extraction
+let serialize32_dsum_known_destr_codom
+  (t: dsum)
+  (k: dsum_known_key t)
+: Tot Type
+= refine_with_tag (dsum_tag_of_data t) (Known k) -> Tot B32.bytes
+
+let serialize32_dsum_known_destr_eq
+  (t: dsum)
+  (k: dsum_known_key t)
+: Tot (serialize32_dsum_known_destr_codom t k -> serialize32_dsum_known_destr_codom t k -> GTot Type0)
+= _ by (T.apply (`feq); T.apply (`eq2))
+
+inline_for_extraction
+let serialize32_dsum_known_destr_if
+  (t: dsum)
+  (k: dsum_known_key t)
+: Tot (if_combinator _ (serialize32_dsum_known_destr_eq t k))
+= fif _ _ _ (default_if _)
+
+#set-options "--z3rlimit 64"
+
+inline_for_extraction
+let serialize32_dsum'
+  (#kt: parser_kind)
+  (t: dsum)
+  (#p: parser kt (dsum_repr_type t))
+  (s: serializer p)
+  (s32: serializer32 (serialize_maybe_enum_key _ s (dsum_enum t)))
+  (f: (x: dsum_known_key t) -> Tot (k: parser_kind & parser k (dsum_type_of_known_tag t x)))
+  (sf: (x: dsum_known_key t) -> Tot (serializer (dsnd (f x))))
+  (sf32: (x: dsum_known_key t) -> Tot (serializer32 (sf x)))
+  (#k': parser_kind)
+  (#g: parser k' (dsum_type_of_unknown_tag t))
+  (#sg: serializer g)
+  (sg32: serializer32 sg)
+  (destr: dep_enum_destr (dsum_enum t) (serialize32_dsum_known_destr_codom t))
+  (u: squash (serializer32_sum_gen_precond kt (weaken_parse_dsum_cases_kind t f k')))
+  (x: dsum_type t)
+: Tot (res: B32.bytes { res == serialize32_dsum_aux t s s32 f sf sf32 sg32 u x } )
+= [@inline_let]
+  let s_tg (tg': dsum_known_key t) (x': refine_with_tag (dsum_tag_of_data t) (Known tg')) : Tot B32.bytes =
+    sf32 tg' (synth_dsum_case_recip t (Known tg') x')
+  in
+  let tg = dsum_tag_of_data t x in
+  let s1 = s32 tg in
+  let s2 =
+    match tg with
+    | Known tg' -> destr (serialize32_dsum_known_destr_eq t) (serialize32_dsum_known_destr_if t) (fun _ _ -> ()) (fun _ _ _ _ -> ()) s_tg tg' x
+    | Unknown _ -> sg32 (synth_dsum_case_recip t tg x)
+  in
+  assert (B32.length s1 + B32.length s2 < 4294967296);
+  let res = s1 `B32.b32append` s2 in
+  assert (res == serialize32_dsum_aux t s s32 f sf sf32 sg32 u x);
+  (res <: (res: B32.bytes { res == serialize32_dsum_aux t s s32 f sf sf32 sg32 u x } ))
+
+
 
 (*
 inline_for_extraction
